refactoring

src/SimulationUtils.v
@@ -1,7 +1,9 @@
+(* TODO: documentation. *)
 Require Import RelationClasses.
 Require Import PathToSubtree.
 From Stdlib Require Import Arith.
 From Stdlib Require Import Relations.
+From Stdlib Require Import Lia.
 
 Arguments clos_refl_trans {_}.
 
@@ -26,94 +28,141 @@ Proof. intros ?. apply rt_refl. Qed.
 Global Instance clos_refl_trans_trans A (R : relation A) : Transitive R^*.
 Proof. intros ?. apply rt_trans. Qed.
 
-(* The general definition of forward simulation. That means that for all a >= b (with
-   a : A and b : B) and a -> c (with c : C), then there exists d : D that completes
-   the following square diagram:
-   b <= a
-   |    |
-   v    v
-   d <= c
-   If A = B and C = D, we call it "preservation".
+Inductive measured_closure {A : Type} (R : nat -> A -> A -> Prop) : nat -> A -> A -> Prop :=
+  | MC_base n x y : R n x y -> measured_closure R n x y
+  | MC_refl n x : measured_closure R n x x
+  | MC_trans m n x y z :
+      measured_closure R m x y -> measured_closure R n y z -> measured_closure R (m + n) x z
+.
 
-   Genarally,
-   - The Leq relations is between states (S <= S'), or pairs of value and state ((v, S) <= (v', S')).
-   - The Red relations are among the following ones:
-     - Evaluation of operands.
-     - Evalutaion of rvalues.
-     - Reorganization.
-     - Evaluation of statements.
+(* Now let's assume that a relation <_n is equipped with an integer measure.
+ * We can define a reflexive-transitive closure that takes the measure into account. *)
+Notation "R ^{ n }" := (measured_closure R n).
+
+Global Instance measured_closure_refl A R n : Reflexive (@measured_closure A R n).
+Proof. intros ?. apply MC_refl. Qed.
+
+Lemma measured_closure_over_approx {A} R m n x y :
+  m <= n -> R^{m} x y -> (@measured_closure A R n x y).
+Proof.
+  intros ? ?. replace n with (m + (n - m)); [ | lia]. eapply MC_trans.
+  - eassumption.
+  - reflexivity.
+Qed.
+
+Definition equiv_rel {A B} (R0 R1 : A -> B -> Prop) := forall a b, R0 a b <-> R1 a b.
+
+Local Instance equiv_rel_refl A B : Reflexive (@equiv_rel A B).
+Proof. intros R a b. reflexivity. Qed.
+
+Lemma measured_closure_equiv A R Rn (H : forall x y : A, R x y <-> exists n, Rn n x y) :
+  forall x y, R^* x y <-> exists n, measured_closure Rn n x y.
+Proof.
+  intros x y. split.
+  - induction 1 as [x y | | x y z ? IH0 ? IH1].
+    + destruct (H x y) as ((n & ?) & _); [assumption | ]. exists n. constructor. assumption.
+    + exists 0. reflexivity.
+    + destruct IH0 as (m & ?). destruct IH1 as (n & ?). exists (m + n).
+      eapply MC_trans; eassumption.
+  - intros (n & G). induction G.
+    + constructor. firstorder.
+    + reflexivity.
+    + etransitivity; eassumption.
+Qed.
+
+(* TODO: name *)
+Lemma measure_closure_cases {A} (R : nat -> A -> A -> Prop) n x z :
+  R^{n} x z -> x = z \/ exists p q y, R^{p} x y /\ R q y z /\ p + q <= n.
+Proof.
+  induction 1 as [n x z | | m n x y z ? IH0 ? IH1].
+  - right. exists 0, n, x. auto using MC_refl.
+  - auto.
+  - destruct IH1 as [-> | (p & q & y' & ? & ? & ?)].
+    + destruct IH0 as [ | (p & q & y & ? & ? & ?)]; [auto | ].
+      right. exists p, q, y. repeat split; try assumption. lia.
+    + right. eexists _, _, y'. repeat split; [ | eassumption | ].
+      * eapply MC_trans; eassumption.
+      * lia.
+Qed.
+
+(** Chaining two relations. *)
+Definition chain {A B C} (RAB : A -> B -> Prop) (RBC : B -> C -> Prop) a c :=
+  exists b, RAB a b /\ RBC b c.
+
+Global Instance reflexive_chain {A} (R S : relation A) `{Reflexive A R} `{Reflexive A S} :
+  Reflexive (chain R S).
+Proof. intros x. exists x. split; reflexivity. Qed.
+
+(* TODO: new documentation. *)
+(* TODO: the direction of the relations LeqAB and LeqCD are the opposite of the diagrams. *)
+(* TODO: The relation RedAC is supposed to be the "right" reduction, and RedBC the "left"
+ * reduction, but these relations are reversed. *)
+(** The general definition of forward simulation. That means that for all [a >= b] (with
+    [a : A] and [b : B]) and [a -> c] (with [c : C]), then there exists [d : D] that completes
+    the following square diagram:
+<<
+b <= a
+|    |
+v    v
+d <= c
+>>
+    If [A = B] and [C = D], we call it "preservation".
+
+    Genarally,
+    - The Leq relations is between states ([S <= S']), or pairs of value and state ([(v, S) <= (v', S')]).
+    - The Red relations are among the following ones:
+      - Evaluation of operands.
+      - Evalutaion of rvalues.
+      - Store operation.
+      - Reorganization.
+      - Evaluation of statements.
  *)
 Definition forward_simulation {A B C D : Type}
   (LeqBA : B -> A -> Prop) (LeqDC : D -> C -> Prop)
   (RedAC : A -> C -> Prop) (RedBD : B -> D -> Prop) :=
   forall a c, RedAC a c -> forall b, LeqBA b a -> exists d, LeqDC d c /\ RedBD b d.
 
-(* To complete a square diagram for HLPL+, we prove that:
-   - The state c reduces to a state c0
-   - The state b is in relation with a state d1: b <= d1
-   - d0 = d1
-   This lemma allows us to not exhibit the terms d0 and d1 explicitely. As the relations LeqCD and
-   RedBD are generally inductively defined, these terms are constructed by applying inductive
-   constructors. This is why the constructors of the relation should be on the form:
-   - red S E[S] for the reduction
-   - E[S] < S for the base relation (only true for HLPL+)
-   Finally, the last goal d0 = d1 is intended to be solved automatically, using the tactic
-   states_eq.
- *)
-Lemma complete_square_diagram {B C D : Type}
-  (LeqDC : D -> C -> Prop) (RedBD : B -> D -> Prop) b c (d0 d1 : D) :
-  LeqDC d0 c -> RedBD b d1 -> d0 = d1
-  -> exists d, LeqDC d c /\ RedBD b d.
-Proof. intros ? ? <-. exists d0. auto. Qed.
+Lemma prove_execution_step {B C D : Type}
+  (LeqDC : D -> C -> Prop) (RedBD : B -> D -> Prop) Sl S'l S'r :
+  RedBD Sl S'l -> LeqDC S'l S'r
+  -> exists S'l, LeqDC S'l S'r /\ RedBD Sl S'l.
+Proof. exists S'l. split; assumption. Qed.
 
-(* To complete a square diagram for LLBC+, we prove that:
-   - The state b is in relation with a state d
-   - The state d reduces to a state c1
-   - c0 = c1
-   This lemma allows us to not exhibit the terms d0 and d1 explicitely. As the relations LeqCD and
-   RedBD are generally inductively defined, these terms are constructed by applying inductive
-   constructors. This is why the constructors of the relation should be on the form:
-   - red S E[S] for the reduction
-   - S < E[S] for the base relation (only true for LLBC+)
-   Finally, the last goal c0 = c1 is intended to be solved automatically, using the tactic
-   states_eq.
- *)
-(* TODO: name *)
-Lemma complete_square_diagram' {B C D : Type}
-  (LeqDC : D -> C -> Prop) (RedBD : B -> D -> Prop) b d c0 c1 :
-  RedBD b d -> LeqDC d c1 -> c0 = c1
-  -> exists d, LeqDC d c0 /\ RedBD b d.
-Proof. intros ? ? <-. exists d. auto. Qed.
+Ltac execution_step := eapply prove_execution_step.
 
-(* Generally, to prove preservation when the relation is a reflexive transitive closure, it
- * suffices to prove it for the base cases. *)
+(** Generally, to prove preservation when the relation is a reflexive transitive closure, it
+    suffices to prove it for the base cases. *)
 Lemma preservation_by_base_case {A B : Type}
-  (LeqA : relation A) (LeqB : relation B) (Red : A -> B -> Prop) :
-  forward_simulation LeqA LeqB^* Red Red ->
-  forward_simulation LeqA^* LeqB^* Red Red.
+  {LeqA : relation A} {LeqB : relation B} `{Reflexive _ LeqB} `{Transitive _ LeqB}
+  {Red : A -> B -> Prop} :
+  forward_simulation LeqA LeqB Red Red ->
+  forward_simulation LeqA^* LeqB Red Red.
 Proof.
-  intros H a b red_ab a' Leq_a_a'. revert b red_ab.
+  intros Hloc a b red_ab a' Leq_a_a'. revert b red_ab.
   induction Leq_a_a' as [ | | a2 a1 a0 _ IH0 _ IH1].
-  - intros. eapply H; eassumption.
-  - intros. eexists. split; [apply rt_refl | eassumption].
+  - intros. eapply Hloc; eassumption.
+  - intros. eexists. split; [reflexivity | eassumption].
   - intros b0 Red_a0_b0.
     destruct (IH1 _ Red_a0_b0) as (b1 & ? & Red_a1_b1).
     destruct (IH0 _ Red_a1_b1) as (b2 & ? & Red_a2_b2).
-    exists b2. split; [ | assumption]. apply rt_trans with (y := b1); assumption.
+    exists b2. split; [ | assumption]. transitivity b1; assumption.
 Qed.
 
-(* Relations are generally defined for types of states, for any semantics between LLBC# and
-   HLPL. In the following section, we will define the relation S <= S' for states,
-   and (v, S) <= (v', S') for pairs of value and state.
-*)
-Class LeqBase state := leq_base : state -> state -> Prop.
-
-(* TODO: is this class useful? *)
-Class WellFormed state := well_formed : state -> Prop.
+(* TODO: define an equivalence between relations? *)
+Lemma forward_simulation_chain {S0 S1} (R0l R0r : S0 -> S0 -> Prop) (R1l R1r : S1 -> S1 -> Prop)
+  (red : S0 -> S1 -> Prop) :
+  forward_simulation R0l R1l red red -> forward_simulation R0r R1r red red ->
+  forward_simulation (chain R0l R0r) (chain R1l R1r) red red.
+Proof.
+  intros Sim_l Sim_r Sr S'r red_Sr_S'r Sl (Sm & R_Sl_Sm & R_Sm_Sr).
+  specialize (Sim_r _ _ red_Sr_S'r _ R_Sm_Sr). destruct Sim_r as (S'm & R_S'm_S'r & red_Sm_S'm).
+  specialize (Sim_l _ _ red_Sm_S'm _ R_Sl_Sm). destruct Sim_l as (S'l & R_S'l_S'm & red_Sl_S'l).
+  exists S'l. split; [ | assumption]. exists S'm. split; assumption.
+Qed.
 
 Section LeqValStateUtils.
   Context `{State state V}.
-  Context `{LB : LeqBase state}.
+  Context (leq_base : state -> state -> Prop).
 
   Definition leq_val_state_base (vSl vSr : V * state) :=
     forall a, fresh_anon (snd vSl) a -> fresh_anon (snd vSr) a ->
@@ -121,7 +170,7 @@ Section LeqValStateUtils.
 
   (* The following two lemmas are used by the tactic `leq_val_state_step`. *)
   Lemma prove_leq_val_state_right_to_left vSl vm Sm vr Sr
-    (G : forall a, fresh_anon Sm a -> fresh_anon Sr a ->
+    (G : forall a, fresh_anon Sr a ->
          exists vSm, leq_base vSm (Sr,, a |-> vr) /\ vSm = Sm,, a |-> vm) :
     leq_val_state_base^* vSl (vm, Sm) ->
     leq_val_state_base^* vSl (vr, Sr).
@@ -131,7 +180,7 @@ Section LeqValStateUtils.
   Qed.
 
   Lemma prove_leq_val_state_left_to_right vl Sl vm Sm vSr
-    (G : forall a, fresh_anon Sm a -> fresh_anon Sl a ->
+    (G : forall a, fresh_anon Sl a ->
          exists vSm, leq_base (Sl,, a |-> vl) vSm /\ vSm = Sm,, a |-> vm) :
     leq_val_state_base^* (vm, Sm) vSr ->
     leq_val_state_base^* (vl, Sl) vSr.
@@ -140,10 +189,23 @@ Section LeqValStateUtils.
     intros a ? ?. cbn in *. destruct (G a) as (? & ? & ->); [assumption.. | ]. assumption.
   Qed.
 
+  Lemma prove_leq_val_state_anon_left vl Sl vm Sm vSr b w
+    (fresh_b : fresh_anon Sl b)
+    (G : forall a, fresh_anon Sl a -> fresh_anon (Sl,, a |-> vl) b ->
+         exists vSm, leq_base (Sl,, a |-> vl,, b |-> w) vSm /\ vSm = Sm,, a |-> vm) :
+    leq_val_state_base^* (vm, Sm) vSr ->
+    leq_val_state_base^* (vl, Sl,, b |-> w) vSr.
+  Proof.
+    intros ?. eapply rt_trans; [ | eassumption]. constructor.
+    intros a (? & ?)%fresh_anon_add_anon ?. cbn in *.
+    rewrite add_anon_commute by congruence.
+    destruct (G a) as (? & ? & ->); try assumption. rewrite fresh_anon_add_anon. auto.
+  Qed.
+
   (* This lemma is used by the tactic `leq_val_state_add_anon`. *)
   Lemma prove_leq_val_state_add_anon vl Sl vm Sm vSr b w
     (fresh_b : fresh_anon Sl b)
-    (G : forall a, fresh_anon Sm a -> fresh_anon Sl a -> fresh_anon (Sl,, a |-> vl) b ->
+    (G : forall a, fresh_anon Sl a -> fresh_anon (Sl,, a |-> vl) b ->
          exists vSm, leq_base (Sl,, a |-> vl) vSm /\ vSm = Sm,, a |-> vm,, b |-> w) :
     leq_val_state_base^* (vm, Sm,, b |-> w) vSr ->
     leq_val_state_base^* (vl, Sl) vSr.
@@ -154,79 +216,195 @@ Section LeqValStateUtils.
     destruct (G a) as (? & ? & ->); try assumption.
     now apply fresh_anon_add_anon.
   Qed.
-
-  (* The issue by directly applying the lemma `preservation_by_base_case` is that it
-     obfuscates the relation le, by unfolding it and replacing it with a reflexive transitive
-     closure.
-     We're going to give similar statements, but these types, the hypothesis uses the relation le.
-   *)
-  (*
-  Lemma preservation_by_base_case_leq_state_leq_val_state
-    (red : state -> (V * state) -> Prop) :
-    forward_simulation E equiv_val_state red red
-    -> forward_simulation (@leq_base _ LB) (@leq _ LeqStateVal) red red
-    -> forward_simulation (clos_refl_trans _ leq_base) LeqStateVal red.
-  Proof. apply preservation_by_base_case. intros ? ? ? ?. reflexivity. Qed.
-   *)
 End LeqValStateUtils.
 
-(* This lemma is used to prove a goal of the form ?vSl < (vr, Sr) or (vl, Sl) < ?vSr without
- * exhibiting the existential variable ?vSl or ?vSr. *)
-Ltac leq_val_state_step :=
-  let a := fresh "a" in
-  lazymatch goal with
-  (* When proving a goal `leq ?vSl (vr, Sr)`, using this tactic creates three subgoals:
-     1. leq_base ?vSm (Sr,, a |-> v)
-     2. ?vSm = ?Sm,, a |-> ?vm
-     3. leq ?vSl (?vm, ?Sm) *)
-  | |- ?leq_star ?vSl (?vr, ?Sr) =>
-      eapply prove_leq_val_state_right_to_left; [intros a ? ?; eexists; split | ]
-  (* When proving a goal `leq (vl, Sl) ?vSr`, using this tactic creates three subgoals:
-     1. leq_base (Sl,, a |-> v) ?vSm
-     2. ?vSm = ?Sm,, a |-> ?vm
-     3. leq (?vm, ?Sm) ?vSr *)
-  (* Note: the hypothesis that a is fresh in ?Sm creates problems.
-     Indeed, ?Sm is an existential and it can be accidently instantiated to a wrong value by
-     eauto. That's why we're removing this hypothesis.
-     TODO: remove it from the hypotheses of the lemma? *)
-  | |- ?leq_star (?vl, ?Sl) ?vSr =>
-      eapply prove_leq_val_state_left_to_right; [intros a _ ?; eexists; split | ]
-(* In either cases:
-   1. Solved by applying the adequate base rule. Here, a is a fresh anon.
-   2. Solved by rewriting (with `autorewrite with spath`) then reflexivity.
-   3. Solved by applying again this tactic, or concluding by reflexivity. *)
-  end.
+Lemma leq_step_right {S} {R : relation S} Sl Sm Sr : R Sm Sr -> R^* Sl Sm -> R^* Sl Sr.
+Proof. intros. transitivity Sm; [ | constructor]; assumption. Qed.
 
-(* In LLBC+, some base rules are of the form S < S',, b |-> w (with b fresh in S). The presence of
- * two anonymous variables, we need to do a special case.
- * Let a be a fresh anon. We prove that
- * 1. Sl,, a |-> vl < ?vSm
- * 2. ?vSm = Sm,, a |-> vm,, b |-> w
- * 3. (?vm, ?Sm) <* ?vSr
- *
- * To apply the base rule in (1), we need a hypothesis that b is fresh in Sl,, a |-> vl. This is
- * true because a and b are two different fresh variables.
- *
- * Because a and b are fresh, we can perform the following commutation:
- * Sm,, a |-> vm,, b |-> w = Sm,, b |-> w,, a |-> vm
- * Using (2), that shows that (vl, Sl) < (vm, Sm,, b |-> w).
- *)
-Ltac leq_val_state_add_anon :=
-  let a := fresh "a" in
-  lazymatch goal with
-  |  |- ?leq_star (?vl, ?Sl) ?vSr =>
-      eapply prove_leq_val_state_add_anon;
-        (* The hypothesis fresh_anon Sl b should be resolved automatically, because there should be
-         * a single hypothesis of the form "fresh_anon Sr b" in the context, with Sr an expression
-         * of Sl, that can be used. *)
-        [eauto with spath; fail |
-         intros a ? ? ?; eexists; split |
-        ]
-  end.
+Lemma leq_step_left {S} {R : relation S} Sl Sm Sr : R Sl Sm -> R^* Sm Sr -> R^* Sl Sr.
+Proof. intros. transitivity Sm; [constructor | ]; assumption. Qed.
+
+(** Tactics to prove commutation of reorganizations. *)
+(* TODO: document it *)
+Lemma prove_reorg_step {S} {reorg leq : relation S} S0 S1 Sr:
+  reorg S0 S1 -> (exists Sl, leq Sl Sr /\ reorg^* S1 Sl) ->
+  exists Sl, leq Sl Sr /\ reorg^* S0 Sl.
+Proof.
+  intros ? (Sl & ? & ?). exists Sl. split; [assumption | ].
+  etransitivity; [constructor | ]; eassumption.
+Qed.
+
+Lemma prove_reorg_steps {S} {reorg leq : relation S} S0 S1 Sr:
+  reorg^* S0 S1 -> (exists Sl, leq Sl Sr /\ reorg^* S1 Sl) ->
+  exists Sl, leq Sl Sr /\ reorg^* S0 Sl.
+Proof.
+  intros ? (Sl & ? & ?). exists Sl. split; [assumption | ].
+  etransitivity; eassumption.
+Qed.
+
+Ltac reorg_step := eapply prove_reorg_step.
+Ltac reorg_steps := eapply prove_reorg_steps.
+Ltac reorg_done := eexists; split; [ | reflexivity].
+
+Section Leq.
+  Context {state : Type}.
+  Context {equiv : state -> state -> Prop}.
+  Context `{Reflexive _ equiv}.
+  Context `{Transitive _ equiv}.
+  Context (leq_base : state -> state -> Prop).
+  Context (sim_leq_base_equiv : forward_simulation leq_base leq_base equiv equiv).
+
+  Definition leq := chain equiv leq_base^*.
+
+  Global Instance reflexive_leq : Reflexive leq.
+  Proof. intros x. exists x. split; reflexivity. Qed.
+
+  Lemma sim_leq_equiv : forward_simulation leq_base^* leq_base^* equiv equiv.
+  Proof.
+    intros a b red_ab a' Leq_a_a'. revert b red_ab.
+    induction Leq_a_a' as [? ? Leq_a_a' | | a2 a1 a0 _ IH0 _ IH1].
+    - intros. specialize (sim_leq_base_equiv _ _ red_ab _ Leq_a_a').
+      destruct sim_leq_base_equiv as (d & ? & ?). exists d. split; [constructor | ]; assumption.
+    - intros. eexists. split; [reflexivity | eassumption].
+    - intros b0 Red_a0_b0.
+      destruct (IH1 _ Red_a0_b0) as (b1 & ? & Red_a1_b1).
+      destruct (IH0 _ Red_a1_b1) as (b2 & ? & Red_a2_b2).
+      exists b2. split; [ | assumption]. transitivity b1; assumption.
+  Qed.
+
+  Global Instance transitive_leq : Transitive leq.
+  Proof.
+    intros x y z (y' & ? & leq_y'_y) (z' & equiv_y_z' & ?).
+    pose proof (sim_leq_equiv _ _ equiv_y_z' _ leq_y'_y) as G.
+    destruct G as (z'' & ? & ?). exists z''. split.
+    - transitivity y'; assumption.
+    - transitivity z'; assumption.
+  Qed.
+
+  Context (reorg : state -> state -> Prop).
+  Context (measure : state -> nat).
+  Context (leq_base_n : nat -> state -> state -> Prop).
+  Definition leq_n n := chain equiv (measured_closure leq_base_n n).
+
+  Hypothesis (leq_decreasing : forall n a b, leq_base_n n a b -> measure a < measure b + n).
+  Hypothesis (reorg_decreasing : forall a b, reorg a b -> measure b < measure a).
+
+  Lemma leq_clos_decreasing : forall S S', reorg^* S S' -> measure S' <= measure S.
+  Proof. intros ? ? Hreorg. induction Hreorg; eauto using Nat.lt_le_incl, Nat.le_trans. Qed.
+
+  Hypothesis (reorg_preserves_equiv : forward_simulation equiv equiv reorg reorg).
+  Lemma reorgs_preserve_equiv : forward_simulation equiv equiv reorg^* reorg^*.
+  Proof.
+  intros a b. induction 1 as [? ? Hreorg | | a0 a1 a2 _ IH0 _ IH1].
+  - intros ? Hequiv. specialize (reorg_preserves_equiv _ _ Hreorg _ Hequiv).
+    destruct reorg_preserves_equiv as (d & ? & ?). exists d.
+    split; [ | constructor]; assumption.
+  - intros. eexists. split; [ | reflexivity]. assumption.
+  - intros b0 equiv_b0_a0.
+    destruct (IH0 _ equiv_b0_a0) as (b1 & Red_b1_a1 & ?).
+    destruct (IH1 _ Red_b1_a1) as (b2 & Red_b2_a1 & ?).
+    exists b2. split; [assumption | ]. transitivity b1; assumption.
+  Qed.
+
+  Context (sim_equiv_leq_base_n :
+    forall n, forward_simulation (leq_base_n n) (leq_base_n n) equiv equiv).
+
+  Lemma leq_n_cases n Sl Sr (G : leq_n n Sl Sr) :
+    (equiv Sl Sr) \/
+    (exists p q Sm, leq_n p Sl Sm /\ leq_base_n q Sm Sr /\ p + q <= n).
+  Proof.
+    destruct G as (Sr' & Gequiv & Gcases%measure_closure_cases).
+    destruct Gcases as [-> | (p & q & Sm & ? & G & ?)].
+    - left. assumption.
+    - right. exists p, q, Sm. firstorder.
+  Qed.
+
+  Lemma sim_equiv_leq_n n : forward_simulation (leq_base_n^{n}) (leq_base_n^{n}) equiv equiv.
+  Proof.
+    intros a b equiv_ab a' Leq_a'_a. revert b equiv_ab.
+    induction Leq_a'_a as [n ? ? Leq_a'_a | | p q a2 a1 a0 _ IH0 _ IH1].
+    - intros. specialize (sim_equiv_leq_base_n n _ _ equiv_ab _ Leq_a'_a).
+      destruct sim_equiv_leq_base_n as (d & ? & ?). exists d. split; [constructor | ]; assumption.
+    - intros. eexists. split; [reflexivity | eassumption].
+    - intros b0 equiv_a0_b0.
+      destruct (IH1 _ equiv_a0_b0) as (b1 & ? & equiv_a1_b1).
+      destruct (IH0 _ equiv_a1_b1) as (b2 & ? & equiv_a2_b2).
+      exists b2. split; [ | assumption]. eapply MC_trans; eassumption.
+  Qed.
+
+  Lemma leq_n_trans Sl Sm Sr p q n :
+    leq_n p Sl Sm -> leq_n q Sm Sr -> p + q <= n -> leq_n n Sl Sr.
+  Proof.
+    intros (S'l & ? & leq_S'l_Sm) (S'm & equiv_Sm_S'm & ?).
+    pose proof (sim_equiv_leq_n p _ _ equiv_Sm_S'm _ leq_S'l_Sm) as (S''l & ? & ?).
+    intros ?. exists S''l. split.
+    - transitivity S'l; assumption.
+    - eapply measured_closure_over_approx; [ eassumption |].
+      eapply MC_trans; eassumption.
+  Qed.
+
+  Lemma measured_preservation_reorg_l
+    (G : forall n, forward_simulation (leq_base_n n) (leq_n n) reorg reorg^*) :
+    forall n, forward_simulation (leq_n n) (leq_n n) reorg^* reorg^*.
+  Proof.
+    intros n Sr. remember (measure Sr + n) as N eqn:EQN.
+    revert n Sr EQN. induction N as [? IH] using lt_wf_ind.
+    intros n Sr -> S''r reorg_Sr_S''r Sl leq_Sl_Sr.
+    destruct reorg_Sr_S''r as [ | Sr S'r S''r reorg_Sr_S'r ? _] using clos_refl_trans_ind_right'.
+    { eexists. split; [eassumption | reflexivity]. }
+    apply leq_n_cases in leq_Sl_Sr.
+    destruct leq_Sl_Sr as [Hequiv | (p & q & Sm & leq_Sl_Sm & leq_Sm_Sr & ?)].
+    { eapply reorgs_preserve_equiv in Hequiv.
+      - destruct Hequiv as (Sl' & ? & ?). exists Sl'. split; [ | assumption].
+        eexists. split; [eassumption | reflexivity].
+      - transitivity S'r; [constructor | ]; assumption. }
+    specialize (G q _ _ reorg_Sr_S'r _ leq_Sm_Sr).
+    destruct G as (S'm & leq_S'm_S'r & reorg_Sm_S'm).
+    specialize (leq_decreasing _ _ _ leq_Sm_Sr).
+    edestruct IH with (Sr := Sm) as (S'l & ? & ?);
+      [ | reflexivity | eassumption.. | ];
+      [lia | ].
+    pose proof (reorg_decreasing _ _ reorg_Sr_S'r).
+    edestruct IH with (Sr := S'r) as (S''m & ? & ?);
+      [ | reflexivity | eassumption.. | ];
+      [lia | ].
+    pose proof (leq_clos_decreasing _ _ reorg_Sm_S'm).
+    edestruct IH with (Sr := S'm) as (S''l & ? & ?);
+      [ | reflexivity | eassumption.. | ]. lia.
+    exists S''l. split.
+    - eapply leq_n_trans; eassumption.
+    - transitivity S'l; assumption.
+  Qed.
+
+  Context (leq_base_is_leq_base_n : forall Sl Sr, leq_base Sl Sr <-> exists n, leq_base_n n Sl Sr).
+
+  Lemma leq_n_is_leq Sl Sr : leq Sl Sr <-> exists n, leq_n n Sl Sr.
+  Proof.
+    split.
+    - intros (Sl' & Hequiv & Hleq).
+      rewrite measured_closure_equiv in Hleq by exact leq_base_is_leq_base_n.
+      destruct Hleq as (n & Hleq). exists n, Sl'. auto.
+    - intros (n & Sl' & Hequiv & Hleq). exists Sl'. split; [assumption | ].
+      rewrite measured_closure_equiv by exact leq_base_is_leq_base_n.
+      exists n. exact Hleq.
+  Qed.
+
+  Corollary preservation_reorg_l
+    (G : forall n, forward_simulation (leq_base_n n) (leq_n n) reorg reorg^*) :
+    forward_simulation leq leq reorg^* reorg^*.
+  Proof.
+    intros Sr S'l reorg_Sr_S'r Sl leq_Sl_Sr.
+    rewrite leq_n_is_leq in leq_Sl_Sr. destruct leq_Sl_Sr as (n & leq_n_Sl_Sr).
+    pose proof (measured_preservation_reorg_l G _ _ _ reorg_Sr_S'r _ leq_n_Sl_Sr)
+      as (Sl' & ? & ?).
+    exists Sl'. split; [ | assumption]. rewrite leq_n_is_leq. exists n. assumption.
+  Qed.
+End Leq.
 
 Section WellFormedSimulations.
-  Context `{LB : LeqBase state}.
-  Context `{WF : WellFormed state}.
+  Context {state : Type}.
+  Context (leq_base : state -> state -> Prop).
+  Context (well_formed : state -> Prop).
 
   (* Preservation of reorgs require well-formedness. However, well-formedness for related states is
    * not proved the same in LLBC+ and HLPL+:
@@ -239,11 +417,6 @@ Section WellFormedSimulations.
     (LeqBA : B -> state -> Prop) (LeqDC : D -> C -> Prop)
     (RedAC : state -> C -> Prop) (RedBD : B -> D -> Prop) :=
     forall a c, well_formed a -> RedAC a c -> forall b, LeqBA b a -> exists d, LeqDC d c /\ RedBD b d.
-
-  Definition well_formed_forward_simulation_l {A C D : Type}
-  (LeqBA : state -> A -> Prop) (LeqDC : D -> C -> Prop)
-  (RedAC : A -> C -> Prop) (RedBD : state -> D -> Prop) :=
-  forall a b c, well_formed b -> RedAC a c -> LeqBA b a -> exists d, LeqDC d c /\ RedBD b d.
 
   (* Reorganizations and leq are defined as reflexive-transitive closure of relations (that we are
    * going to denote < and reorg). When we want to prove the preservation, ie:
@@ -270,14 +443,13 @@ Section WellFormedSimulations.
    * However, this proof scheme is wrong in general. Our strategy is to exhibit a measure |.| from
    * states to a well-founded order, that is decreasing by applications of < and reorg.
    *)
-  (* Note: for the moment, we just use natural measures. *)
   Lemma preservation_reorg_r (reorg : state -> state -> Prop)
     (measure : state -> nat)
     (leq_decreasing : forall a b, leq_base a b -> measure a < measure b)
     (reorg_decreasing : forall a b, reorg a b -> measure b < measure a)
     (leq_base_preserves_wf_r : forall a b, well_formed b -> leq_base a b -> well_formed a)
-    (reorg_preserves_wf : forall a b, reorg a b -> @well_formed _ WF a -> @well_formed _ WF b)
-    (H : well_formed_forward_simulation_r (@leq_base _ LB) (@leq_base _ LB)^* reorg reorg^*) :
+    (reorg_preserves_wf : forall a b, reorg a b -> well_formed a -> well_formed b)
+    (H : well_formed_forward_simulation_r leq_base leq_base^* reorg reorg^*) :
     well_formed_forward_simulation_r leq_base^* leq_base^* reorg^* reorg^*.
   Proof.
     (* Sequences of reorgenizations make the measure decrease. *)
@@ -301,43 +473,6 @@ Section WellFormedSimulations.
       as (Sm'' & ? & ?)
       by eauto.
     assert (exists Sl'', leq_base^* Sl'' Sm'' /\ reorg^* Sl' Sl'')
-      as (? & ? & ?).
-    { eapply IH; [ | reflexivity | | eassumption..]; eauto using Nat.le_lt_trans. }
-    eexists. split; eapply rt_trans; eassumption.
-  Qed.
-
-  Lemma preservation_reorg_l (reorg : state -> state -> Prop)
-    (measure : state -> nat)
-    (leq_decreasing : forall a b, leq_base a b -> measure a < measure b)
-    (reorg_decreasing : forall a b, reorg a b -> measure b < measure a)
-    (leq_base_preserves_wf_l : forall a b, well_formed a -> leq_base a b -> well_formed b)
-    (reorg_preserves_wf : forall a b, reorg a b -> @well_formed _ WF a -> @well_formed _ WF b)
-    (H : well_formed_forward_simulation_l (@leq_base _ LB) (@leq_base _ LB)^* reorg reorg^*) :
-    well_formed_forward_simulation_l leq_base^* leq_base^* reorg^* reorg^*.
-  Proof.
-    assert (forall S S', reorg^* S S' -> measure S' <= measure S).
-    { intros ? ? Hreorg. induction Hreorg; eauto using Nat.lt_le_incl, Nat.le_trans. }
-    assert (forall S S', well_formed S -> reorg^* S S' -> well_formed S').
-    { intros ? ? ? Hreorg. induction Hreorg; eauto. }
-    assert (forall Sl Sr, well_formed Sl -> leq_base^* Sl Sr -> well_formed Sr).
-    { intros ? ? ? G. induction G; eauto. }
-    intros Sr.
-    remember (measure Sr) as n eqn:EQN. revert Sr EQN.
-    induction n as [? IH] using lt_wf_ind.
-    intros Sr -> Sl Sr' well_formed_Sl reorg_Sr_Sr'.
-    destruct reorg_Sr_Sr' as [ | Sr Sr' Sr'' reorg_Sr_Sr' ? _] using clos_refl_trans_ind_right'.
-    { intros. eexists. split; [eassumption | apply rt_refl]. }
-    intros leq_Sl_Sr.
-    destruct leq_Sl_Sr as [ | Sl Sm Sr ? _ leq_Sm_Sr] using clos_refl_trans_ind_left'.
-    { eexists. split; [apply rt_refl | ]. eapply rt_trans; [constructor | ]; eassumption. }
-    destruct (H Sr Sm Sr') as (Sm' & leq_Sm'_Sr' & reorg_Sm_Sm'); [eauto.. | ].
-    assert (exists Sl', leq_base^* Sl' Sm' /\ clos_refl_trans reorg Sl Sl')
-      as (Sl' & ? & ?)
-      by eauto.
-    assert (exists Sm'', leq_base^* Sm'' Sr'' /\ clos_refl_trans reorg Sm' Sm'')
-      as (Sm'' & ? & ?)
-      by eauto.
-    assert (exists Sl'', leq_base^* Sl'' Sm'' /\ clos_refl_trans reorg Sl' Sl'')
       as (? & ? & ?).
     { eapply IH; [ | reflexivity | | eassumption..]; eauto using Nat.le_lt_trans. }
     eexists. split; eapply rt_trans; eassumption.
